Incorrectness/Assert.lean
@@ -1,0 +1,14 @@
+import Incorrectness.Defs
+open Language
+namespace Incorrectness
+
+theorem assert_intro {P : State → Prop} {B : State → Prop} :
+    [* fun s => P s ∧ B s *] (Stmt.assert B) [* fun s => P s ∧ B s *] := by
+  intro t hPost
+  obtain ⟨hPt, hBt⟩ := hPost
+  exists t
+  constructor
+  · exact ⟨hPt, hBt⟩
+  · exact BigStep.assert B t hBt
+
+end Incorrectness
